Start removing nearly redundant ILs
conLang, dewcLang and exhLang didn't differ much from modLang, and with
the relocation of the match exhaustiveness to modLang, there wasn't much
reason to keep them. Some files ruthlessly commented out to get things
to build.

compiler/backend/mod_reorder_matchScript.sml
@@ -1,6 +1,6 @@
-open preamble exhLangTheory
+open preamble modLangTheory
 
-val _ = new_theory"exh_reorder";
+val _ = new_theory"mod_reorder_exn";
 
 val is_const_con_def = Define`
   (is_const_con (Pcon tag plist) = (plist = [])) /\
@@ -69,6 +69,7 @@ val compile_def = tDefine "compile" `
     (compile [Var_global t n] = [Var_global t n]) /\
     (compile [Fun t v e] = [Fun t v (HD (compile [e]))]) /\
     (compile [App t op es] = [App t op (compile es)]) /\
+    (compile [If t e1 e2 e3] = [If t (HD (compile [e1])) (HD (compile [e2])) (HD (compile [e3]))]) ∧
     (compile [Mat t e pes] =  [Mat t (HD (compile [e])) (MAP (λ(p,e). (p,HD (compile [e]))) (const_cons_fst pes))]) /\
     (compile [Let t vo e1 e2] = [Let t vo (HD (compile [e1])) (HD (compile [e2]))]) /\
     (compile [Letrec t funs e] =
@@ -102,15 +103,15 @@ val compile_ind = theorem"compile_ind";
 val compile_length = Q.store_thm ("compile_length[simp]",
   `! es. LENGTH (compile es) = LENGTH es`,
   ho_match_mp_tac compile_ind
-  \\ rw [compile_def])
+  \\ rw [compile_def]);
 
 val compile_sing = Q.store_thm ("compile_sing",
   `! e. ?e2. compile [e] = [e2]`,
   rw []
   \\ qspec_then `[e]` mp_tac compile_length
-  \\ simp_tac(std_ss++listSimps.LIST_ss)[LENGTH_EQ_NUM_compute])
+  \\ simp_tac(std_ss++listSimps.LIST_ss)[LENGTH_EQ_NUM_compute]);
 
-val compile_nil = save_thm ("compile_nil[simp]", EVAL ``exh_reorder$compile []``);
+val compile_nil = save_thm ("compile_nil[simp]", EVAL ``compile []``);
 
 val compile_cons = Q.store_thm ("compile_cons",
   `! e es. compile (e::es) = HD (compile [e]) :: (compile es)`,
