compiler/backend/mod_to_patScript.sml
@@ -1,7 +1,7 @@
-open preamble exhLangTheory patLangTheory
+open preamble modLangTheory patLangTheory
 open backend_commonTheory
 
-val _ = new_theory"exh_to_pat"
+val _ = new_theory"mod_to_pat"
 val _ = patternMatchesLib.ENABLE_PMATCH_CASES();
 
 val Bool_def = Define `
@@ -67,7 +67,7 @@ val _ = Define `
     (!n. op <> FFI n)`;
 
 val _ = Define `
-  (pure_op (Op (Op op)) ⇔ pure_op_op op)
+  (pure_op (Op op) ⇔ pure_op_op op)
   ∧
   (pure_op (Op (Init_global_var _)) ⇔ F)
   ∧
@@ -243,18 +243,18 @@ val _ = tDefine"compile_pat"`
    Bool t T)
   ∧
   (compile_pat t (Plit l) =
-   App (mk_cons t 1) (Op (Op Equality)) [Var_local (mk_cons t 2) 0; Lit (mk_cons t 3) l])
+   App (mk_cons t 1) (Op Equality) [Var_local (mk_cons t 2) 0; Lit (mk_cons t 3) l])
   ∧
-  (compile_pat t (Pcon tag []) =
+  (compile_pat t (Pcon (SOME (tag,_)) []) =
    App (mk_cons t 1) (Tag_eq tag 0) [Var_local (mk_cons t 2) 0])
   ∧
-  (compile_pat t (Pcon tag ps) =
+  (compile_pat t (Pcon (SOME (tag,_)) ps) =
    sIf (mk_cons t 1) (App (mk_cons t 2) (Tag_eq tag (LENGTH ps)) [Var_local (mk_cons t 3) 0])
      (Let_Els (mk_cons t 4) 0 (LENGTH ps) (compile_pats (mk_cons t 5) 0 ps))
      (Bool (mk_cons t 6) F))
   ∧
   (compile_pat t (Pref p) =
-   sLet (mk_cons t 1) (App (mk_cons t 2) (Op (Op Opderef)) [Var_local (mk_cons t 3) 0])
+   sLet (mk_cons t 1) (App (mk_cons t 2) (Op Opderef) [Var_local (mk_cons t 3) 0])
      (compile_pat (mk_cons t 4) p))
   ∧
 (* return an expression that evaluates to whether all the m patterns match the
@@ -283,7 +283,7 @@ val _ = tDefine"compile_row"`
   ∧
   (compile_row t bvs (Pref p) =
    let (bvs,m,f) = (compile_row (mk_cons t 1) (NONE::bvs) p) in
-   (bvs,(1+m), (λe. sLet (mk_cons t 2) (App (mk_cons t 3) (Op (Op Opderef)) [Var_local (mk_cons t 4) 0]) (f e)))) ∧
+   (bvs,(1+m), (λe. sLet (mk_cons t 2) (App (mk_cons t 3) (Op Opderef) [Var_local (mk_cons t 4) 0]) (f e)))) ∧
   (compile_row _ bvs _ = (bvs, 0, I)) (* should not happen *)
   ∧
   (compile_cols _ bvs _ _ [] = (bvs, 0, I))
@@ -306,7 +306,7 @@ val compile_exp_def = tDefine"compile_exp" `
   ∧
   (compile_exp _ (Lit t l) = Lit t l)
   ∧
-  (compile_exp bvs (Con t tag es) = Con t tag (compile_exps bvs es))
+  (compile_exp bvs (Con t (SOME (tag,_)) es) = Con t tag (compile_exps bvs es))
   ∧
   (compile_exp bvs (Var_local t x) =
    (dtcase find_index (SOME x) bvs 0 of
